backend/LTL.v
@@ -303,14 +303,14 @@ Definition set_mem (s:state) (m:mem):=
   | Returnstate sf ls _ => Returnstate sf ls m
   end.
 
-Parameter initial_core: program -> mem -> state -> val -> list val -> Prop.
+Parameter entry_point: program -> mem -> state -> val -> list val -> Prop.
 Parameter at_external : state -> option (external_function * signature * list val).
 Parameter after_external : option val -> state -> Memory.mem -> option state.
 
 Definition semantics (p: program) :=
   let main :=p.(prog_main) in
   let init_mem:=(Genv.init_mem p) in
-  Semantics get_mem set_mem step (initial_core p) at_external after_external final_state (Genv.globalenv p) main init_mem.
+  Semantics get_mem set_mem step (entry_point p) at_external after_external final_state (Genv.globalenv p) main init_mem.
 
 (** * Operations over LTL *)
 
